lean-formalisation/LeanFormalisation/LBase/LBaseCFG/Framework.lean
@@ -20,41 +20,40 @@ class Framework
     (A : Type) [Bot A] [Max A] [FiniteHeight A]
     (edgeTransfer : CFGEdge -> A -> A)
     (nodeTransfer : CFGNode -> A -> A)
-    (s : Lang .Stmt) (R : StateRel)
+    (s : Lang .Stmt) (R : StateRel) [TranslationReq s R]
     (abs : CEK -> A -> Prop)
     extends LatticeLike A nodeTransfer edgeTransfer where
-
+  entryInit : A
+  init_sound : abs (initState s) entryInit
   abs_mono : ∀ {σ : CEK} {a b : A}, a ⊔ b = b -> abs σ a -> abs σ b
   abs_preserves_init : ∀ {a : A}, abs (initState s) a ->
     abs (initState s) (nodeTransfer (stmtCFG s).entry a)
-
-  step_sound : ∀ {σ σ' : CEK} {n n' : CFGNode} {entryInit : A},
+  step_sound : ∀ {σ σ' : CEK} {n n' : NodeOf (stmtCFG s)},
     R σ n -> R σ' n' -> Eval σ σ' -> CFGReach (stmtCFG s) n n' ->
-    ∀ (f : fact A), IsForwardPostFixpoint (stmtCFG s) nodeTransfer edgeTransfer entryInit f ->
+    ∀ (f : GFact (stmtCFG s) A),
+      IsForwardPostFixpointOf (stmtCFG s) nodeTransfer edgeTransfer entryInit f ->
     abs σ (f n) -> abs σ' (f n')
 
 /-- for all reachable CEK states σ, there exists a state n such that -/
-theorem dataflow_soundness_exists {s : Lang .Stmt}
+theorem worklistForwardEdgeOf_soundness_exists {s : Lang .Stmt}
     {A : Type} [Bot A] [Max A] [DecidableEq A] [FiniteHeight A]
     {edgeTransfer : CFGEdge -> A -> A} {nodeTransfer : CFGNode -> A -> A}
     {abs : CEK -> A -> Prop} {R : StateRel} [tr : TranslationReq s R]
     [fr : Framework A edgeTransfer nodeTransfer s R abs]
-    (entryInit : A) (out0 : fact A)
-    (wl0 : List CFGNode) (hwl0 : ∀ x ∈ wl0, x ∈ (stmtCFG s).nodes)
-    (h_inv0 : ∀ m, m ∉ wl0 ->
-        nodeTransfer m (expectedIn (stmtCFG s) edgeTransfer entryInit out0 m) ⊔ out0 m = out0 m)
-    (hinit_sound : abs (initState s) entryInit)
     (σ : CEK) (hreach : CEKReach (initState s) σ) :
-    let res := worklistForwardEdge (stmtCFG s) nodeTransfer edgeTransfer entryInit out0 wl0 hwl0
-    ∃ n, R σ n ∧ abs σ (res n) := by
+    let res := worklistForwardEdgeOf (stmtCFG s) nodeTransfer edgeTransfer fr.entryInit
+    ∃ n : NodeOf (stmtCFG s), R σ n ∧ abs σ (res n) := by
   intro res
-  have h_postfix : IsForwardPostFixpoint (stmtCFG s) nodeTransfer edgeTransfer entryInit res :=
-    worklist_sound_postfixpoint (stmtCFG s) nodeTransfer edgeTransfer entryInit out0 wl0 hwl0 h_inv0
+  have h_postfix : IsForwardPostFixpointOf (stmtCFG s) nodeTransfer edgeTransfer fr.entryInit res :=
+    worklistForwardEdgeOf_sound_postfixpoint (stmtCFG s) nodeTransfer edgeTransfer fr.entryInit
+      (fun _ => ⊥) ((stmtCFG s).nodes_mem) (by grind only [CFG.nodes_mem, usr List.mem_pmap_of_mem])
   induction hreach with
   | refl =>
-    refine ⟨(stmtCFG s).entry, tr.init_related, ?_⟩
-    refine fr.abs_mono ?_ (fr.abs_preserves_init hinit_sound)
-    simpa [expectedIn] using h_postfix (stmtCFG s).entry
+    let nen : NodeOf (stmtCFG s) := ⟨(stmtCFG s).entry, (stmtCFG s).entry_in_nodes⟩
+    let nex : NodeOf (stmtCFG s) := ⟨(stmtCFG s).exit, (stmtCFG s).exit_in_nodes⟩
+    refine ⟨nen, tr.init_related, ?_⟩
+    refine fr.abs_mono ?_ (fr.abs_preserves_init fr.init_sound)
+    simpa [expectedInOf, nen] using h_postfix nen
   | tail σ_mid h_eval ih =>
     obtain ⟨n, hstep, habs⟩ := ih
     obtain ⟨n', hstep', habs'⟩ := tr.step_sound hstep h_eval
@@ -62,32 +61,66 @@ theorem dataflow_soundness_exists {s : Lang .Stmt}
     apply fr.step_sound hstep hstep' h_eval habs' res h_postfix
     grind
 
-theorem dataflow_soundness {s : Lang .Stmt}
+/-- for all reachable CEK states σ, there exists a state n such that -/
+theorem dataflow_soundness_exists {s : Lang .Stmt}
     {A : Type} [Bot A] [Max A] [DecidableEq A] [FiniteHeight A]
     {edgeTransfer : CFGEdge -> A -> A} {nodeTransfer : CFGNode -> A -> A}
     {abs : CEK -> A -> Prop} {R : StateRel} [tr : TranslationReq s R]
     [fr : Framework A edgeTransfer nodeTransfer s R abs]
-    (entryInit : A) (out0 : fact A)
-    (wl0 : List CFGNode) (hwl0 : ∀ x ∈ wl0, x ∈ (stmtCFG s).nodes)
-    (h_inv0 : ∀ m, m ∉ wl0 ->
-        nodeTransfer m (expectedIn (stmtCFG s) edgeTransfer entryInit out0 m) ⊔ out0 m = out0 m)
-    (hinit_sound : abs (initState s) entryInit)
-    (σ : CEK) (n : CFGNode) (hreach : CEKReach (initState s) σ) (hrel : R σ n) :
-    let res := worklistForwardEdge (stmtCFG s) nodeTransfer edgeTransfer entryInit out0 wl0 hwl0
+    (σ : CEK) (hreach : CEKReach (initState s) σ) :
+    let data := runDataflowOf (stmtCFG s) nodeTransfer edgeTransfer fr.entryInit
+    ∃ n : NodeOf (stmtCFG s), R σ n ∧ abs σ (data.2 n) := by
+  intro data
+  exact worklistForwardEdgeOf_soundness_exists σ hreach
+
+lemma IsForwardFixpointOf.to_postfixpoint {A : Type} [Bot A] [Max A] [FiniteHeight A]
+    (g : CFG) (nodeTransfer : CFGNode -> A -> A) (edgeTransfer : CFGEdge -> A -> A)
+    (outF : GFact g A) [ll : LatticeLike A nodeTransfer edgeTransfer]
+    (entryInit : A)
+    (hfix : IsForwardFixpointOf g nodeTransfer edgeTransfer entryInit outF) :
+    IsForwardPostFixpointOf g nodeTransfer edgeTransfer entryInit outF := by
+  intro n
+  rw [hfix n]
+  simp [ll.join_idem]
+
+theorem worklistForwardEdgeOf_soundness {s : Lang .Stmt}
+    {A : Type} [Bot A] [Max A] [DecidableEq A] [FiniteHeight A]
+    {edgeTransfer : CFGEdge -> A -> A} {nodeTransfer : CFGNode -> A -> A}
+    {abs : CEK -> A -> Prop} {R : StateRel} [tr : TranslationReq s R]
+    [fr : Framework A edgeTransfer nodeTransfer s R abs]
+    (σ : CEK) (n : NodeOf (stmtCFG s))
+    (hreach : CEKReach (initState s) σ) (hrel : R σ n) :
+    let res := worklistForwardEdgeOf (stmtCFG s) nodeTransfer edgeTransfer fr.entryInit
     abs σ (res n) := by
   intro res
-  have h_postfix : IsForwardPostFixpoint (stmtCFG s) nodeTransfer edgeTransfer entryInit res :=
-    worklist_sound_postfixpoint (stmtCFG s) nodeTransfer edgeTransfer entryInit out0 wl0 hwl0 h_inv0
+  have h_postfix :
+      IsForwardPostFixpointOf (stmtCFG s) nodeTransfer edgeTransfer fr.entryInit res := by
+    have := (worklistForwardEdgeOf_sound_fixpoint (stmtCFG s) nodeTransfer edgeTransfer fr.entryInit
+      (fun _ => ⊥) ((stmtCFG s).nodes_mem) (by grind only [CFG.nodes_mem, usr List.mem_pmap_of_mem])
+        (by grind [fr.join_comm, fr.bot_le]))
+    exact this.to_postfixpoint
   induction hreach generalizing n with
   | refl =>
-    unfold IsForwardPostFixpoint at h_postfix
+    unfold IsForwardPostFixpointOf at h_postfix
     have : n = (stmtCFG s).entry := tr.init_uniq hrel
     apply fr.abs_mono (h_postfix n)
-    simp only [this, expectedIn, ↓reduceIte]
+    simp only [this, expectedInOf, ↓reduceIte]
     apply fr.abs_preserves_init
-    assumption
+    exact fr.init_sound
   | tail hreach h_eval ih =>
     rename_i σ_mid σ'
     have ⟨nmid, hr_mid, hreach_mid⟩ := tr.step_complete h_eval hrel
     specialize ih nmid hr_mid
     grind [fr.step_sound]
+
+theorem dataflow_soundness {s : Lang .Stmt}
+    {A : Type} [Bot A] [Max A] [DecidableEq A] [FiniteHeight A]
+    {edgeTransfer : CFGEdge -> A -> A} {nodeTransfer : CFGNode -> A -> A}
+    {abs : CEK -> A -> Prop} {R : StateRel} [tr : TranslationReq s R]
+    [fr : Framework A edgeTransfer nodeTransfer s R abs]
+    (σ : CEK) (n : NodeOf (stmtCFG s))
+    (hreach : CEKReach (initState s) σ) (hrel : R σ n) :
+    let data := runDataflowOf (stmtCFG s) nodeTransfer edgeTransfer fr.entryInit
+    abs σ (data.2 n) := by
+  intro data
+  exact worklistForwardEdgeOf_soundness σ n hreach hrel
